\documentclass[12pt]{article}
 
\usepackage[margin=0.8in]{geometry}
\usepackage{amsmath,amsthm,amssymb}

\title{Answer Sheet: Factoring Polynomials Homework}
\author{\today}
\date{}
\begin{document}

\maketitle

\section*{Answers}

\begin{enumerate}
    \item Factor the following quadratic equations using the factoring method discussed in class.
    \begin{enumerate}
        \item $8x^2 + 22x + 15 = 0$
        \begin{align*}
            A \times C & = 8 \times 15 = 120 \\
            \text{Factors of 120 that add up to 22:} & \quad 10 \text{ and } 12 \\
            8x^2 + 10x + 12x + 15 &= 0 \\
            2x(4x + 5) + 3(4x + 5) &= 0 \\
            (4x + 5)(2x + 3) &= 0
        \end{align*}
        
        \item $3x^2 + 11x + 6 = 0$
        \begin{align*}
            A \times C & = 3 \times 6 = 18 \\
            \text{Factors of 18 that add up to 11:} & \quad 9 \text{ and } 2 \\
            3x^2 + 9x + 2x + 6 &= 0 \\
            3x(x + 3) + 2(x + 3) &= 0 \\
            (x + 3)(3x + 2) &= 0
        \end{align*}
        
        \item $7x^2 + 19x + 6 = 0$
        \begin{align*}
            A \times C & = 7 \times 6 = 42 \\
            \text{Factors of 42 that add up to 19:} & \quad 14 \text{ and } 3 \\
            7x^2 + 14x + 3x + 6 &= 0 \\
            7x(x + 2) + 3(x + 2) &= 0 \\
            (x + 2)(7x + 3) &= 0
        \end{align*}
        
        \item $6x^2 + 17x + 12 = 0$
        \begin{align*}
            A \times C & = 6 \times 12 = 72 \\
            \text{Factors of 72 that add up to 17:} & \quad 9 \text{ and } 8 \\
            6x^2 + 9x + 8x + 12 &= 0 \\
            3x(2x + 3) + 4(2x + 3) &= 0 \\
            (2x + 3)(3x + 4) &= 0
        \end{align*}
        
        \item $5x^2 + 16x + 12 = 0$
        \begin{align*}
            A \times C & = 5 \times 12 = 60 \\
            \text{Factors of 60 that add up to 16:} & \quad 10 \text{ and } 6 \\
            5x^2 + 10x + 6x + 12 &= 0 \\
            5x(x + 2) + 6(x + 2) &= 0 \\
            (x + 2)(5x + 6) &= 0
        \end{align*}
    \end{enumerate}

    \item Solve the following quadratic equations by factoring.
    \begin{enumerate}
        \item $2x^2 + 9x + 7 = 0$
        \begin{align*}
            A \times C & = 2 \times 7 = 14 \\
            \text{Factors of 14 that add up to 9:} & \quad 7 \text{ and } 2 \\
            2x^2 + 7x + 2x + 7 &= 0 \\
            x(2x + 7) + 1(2x + 7) &= 0 \\
            (2x + 7)(x + 1) &= 0 \\
            \text{Solutions: } x &= -\frac{7}{2}, -1
        \end{align*}
        
        \item $4x^2 + 15x + 9 = 0$
        \begin{align*}
            A \times C & = 4 \times 9 = 36 \\
            \text{Factors of 36 that add up to 15:} & \quad 12 \text{ and } 3 \\
            4x^2 + 12x + 3x + 9 &= 0 \\
            4x(x + 3) + 3(x + 3) &= 0 \\
            (x + 3)(4x + 3) &= 0 \\
            \text{Solutions: } x &= -3, -\frac{3}{4}
        \end{align*}
        
        \item $9x^2 + 30x + 21 = 0$
        \begin{align*}
            A \times C & = 9 \times 21 = 189 \\
            \text{Factors of 189 that add up to 30:} & \quad 21 \text{ and } 9 \\
            9x^2 + 21x + 9x + 21 &= 0 \\
            3x(3x + 7) + 3(3x + 7) &= 0 \\
            (3x + 7)(3x + 3) &= 0 \\
            \text{Solutions: } x &= -\frac{7}{3}, -1
        \end{align*}
        
        \item $12x^2 + 23x + 10 = 0$
        \begin{align*}
            A \times C & = 12 \times 10 = 120 \\
            \text{Factors of 120 that add up to 23:} & \quad 15 \text{ and } 8 \\
            12x^2 + 15x + 8x + 10 &= 0 \\
            3x(4x + 5) + 2(4x + 5) &= 0 \\
            (4x + 5)(3x + 2) &= 0 \\
            \text{Solutions: } x &= -\frac{5}{4}, -\frac{2}{3}
        \end{align*}
        
        \item $10x^2 + 27x + 18 = 0$
        \begin{align*}
            A \times C & = 10 \times 18 = 180 \\
            \text{Factors of 180 that add up to 27:} & \quad 15 \text{ and } 12 \\
            10x^2 + 15x + 12x + 18 &= 0 \\
            5x(2x + 3) + 6(2x + 3) &= 0 \\
            (2x + 3)(5x + 6) &= 0 \\
            \text{Solutions: } x &= -\frac{3}{2}, -\frac{6}{5}
        \end{align*}
    \end{enumerate}

    \item For each of the following quadratic equations, verify your factored form by expanding back to the original polynomial.
    \begin{enumerate}
        \item $6x^2 + 13x + 6 = 0$
        \begin{align*}
            (2x + 3)(3x + 2) &= 6x^2 + 4x + 9x + 6 \\
            &= 6x^2 + 13x + 6
        \end{align*}
        
        \item $8x^2 + 14x + 3 = 0$
        \begin{align*}
            (4x + 1)(2x + 3) &= 8x^2 + 12x + 2x + 3 \\
            &= 8x^2 + 14x + 3
        \end{align*}
        
        \item $5x^2 + 24x + 16 = 0$
        \begin{align*}
            (x + 8)(5x + 2) &= 5x^2 + 2x + 40x + 16 \\
            &= 5x^2 + 24x + 16
        \end{align*}
        
        \item $3x^2 + 19x + 20 = 0$
        \begin{align*}
            (3x + 4)(x + 5) &= 3x^2 + 15x + 4x + 20 \\
            &= 3x^2 + 19x + 20
        \end{align*}
        
        \item $7x^2 + 31x + 20 = 0$
        \begin{align*}
            (x + 4)(7x + 5) &= 7x^2 + 5x + 28x + 20 \\
            &= 7x^2 + 31x + 20
        \end{align*}
    \end{enumerate}

    \item Challenge problems: Factor the following quadratic equations where the leading coefficient is not 1.
    \begin{enumerate}
        \item $9x^2 + 24x + 16 = 0$
        \begin{align*}
            A \times C & = 9 \times 16 = 144 \\
            \text{Factors of 144 that add up to 24:} & \quad 12 \text{ and } 12 \\
            9x^2 + 12x + 12x + 16 &= 0 \\
            3x(3x + 4) + 4(3x + 4) &= 0 \\
            (3x + 4)(3x + 4) &= 0
        \end{align*}
        
        \item $12x^2 + 25x + 12 = 0$
        \begin{align*}
            A \times C & = 12 \times 12 = 144 \\
            \text{Factors of 144 that add up to 25:} & \quad 9 \text{ and } 16 \\
            12x^2 + 9x + 16x + 12 &= 0 \\
            3x(4x + 3) + 4(4x + 3) &= 0 \\
            (4x + 3)(3x + 4) &= 0
        \end{align*}
        
        \item $15x^2 + 26x + 8 = 0$
        \begin{align*}
            A \times C & = 15 \times 8 = 120 \\
            \text{Factors of 120 that add up to 26:} & \quad 10 \text{ and } 12 \\
            15x^2 + 10x + 12x + 8 &= 0 \\
            5x(3x + 2) + 4(3x + 2) &= 0 \\
            (3x + 2)(5x + 4) &= 0
        \end{align*}
    \end{enumerate}
\end{enumerate}

\end{document}